\section{Translation}

\begin{align*}
	(\Sigma,R,H,P)^+ & \rightarrow (\Sigma,R,H^*,P) \\
	(\Sigma,R,H,P)^? & \rightarrow (\Sigma,R,H^{**},P) 
\end{align*}

\begin{align*}
	(H_1 \land H_2)^* & \rightarrow H_1^* \land H_2^* \\
	(H_1 \lor H_2)^* & \rightarrow H_1^* \lor H_2^* \\
	(r_i.a_i = c_i)^* & \rightarrow r_i.a_i = c_i \\
	(r_i.a_i \neq c_i)^*& \rightarrow r_i.a_i \neq c_i \\
	(r_i.a_i = r_j.a_j)^* & \rightarrow r_i.a_i = r_j.a_j \\
	(r_i.a_i \neq r_j.a_j)^* & \rightarrow r_i.a_i \neq r_j.a_j \\
	null(r_i.a_i)^* & \rightarrow null(r_i.a_i) \\
	const(r_i.a_i)^* & \rightarrow const(r_i.a_i) \\
	exists(Q)^* & \rightarrow exists(Q^+) \\
	notexists(Q)^* & \rightarrow notexists(Q^?) \\
	in(r_i.a_i,Q)^* & \rightarrow in(r_i.a_i,Q^+) \\
	notin(r_i.a_i,Q)^* & \rightarrow notin(r_i.a_i,Q^?) 
\end{align*}

\begin{align*}
	(H_1 \land H_2)^{**} & \rightarrow H_1^{**} \land H_2^{**} \\
	(H_1 \lor H_2)^{**} & \rightarrow H_1^{**} \lor H_2^{**} \\
	(r_i.a_i = c_i)^{**} & \rightarrow r_i.a_i = c_i \lor null(r_i.a_i)\\
	(r_i.a_i \neq c_i)^{**}& \rightarrow r_i.a_i \neq c_i \lor null(r_i.a_i)\\
	(r_i.a_i = r_j.a_j)^{**} & \rightarrow r_i.a_i = r_j.a_j \lor null(r_i.a_i) \lor null(r_j.a_j)\\
	(r_i.a_i \neq r_j.a_j)^{**} & \rightarrow r_i.a_i \neq r_j.a_j  \lor null(r_i.a_i) \lor null(r_j.a_j)\\
	null(r_i.a_i)^{**} & \rightarrow null(r_i.a_i) \\
	const(r_i.a_i)^{**} & \rightarrow const(r_i.a_i) \\
	exists(Q)^{**} & \rightarrow exists(Q^?) \\
	notexists(Q)^{**} & \rightarrow notexists(Q^+) \\
	in(r_i.a_i,Q)^{**} & \rightarrow in(r_i.a_i,Q^?) \\
	notin(r_i.a_i,Q)^{**} & \rightarrow notin(r_i.a_i,Q^+) 
\end{align*}

\begin{myprop}
	$$\forall Q \in \llbracket SQL \rrbracket, Eval_{SQL}(Q^+,D) \subseteq cert_\bot(Q,D)$$
\end{myprop}
\begin{myprop}
	$$\forall Q \in \llbracket SQL \rrbracket, posi_\bot(Q,D) = \{ x | \exists h, h(x) \in  Eval_{SQL}(Q,h(D)) \} \subseteq Eval_{SQL}(Q^?,D)$$
\end{myprop}

\begin{proof}
	Assume (5).
	\\By induction ...
	\begin{align*}
		x \in Eval_{SQL}((\Sigma,R,notexists(Q),P)^+,D) &\Rightarrow x \in Eval_{SQL}((\Sigma,R,notexists(Q^?),P),D) \\
		&\Rightarrow Eval_{SQL}(Q^?[x],D) = \emptyset \\
		&\Rightarrow \{ y | \exists h, h(y) \in  Eval_{SQL}(Q[h(x)],h(D)) \} = \emptyset \mbox{ (by 5)}\\
		&\Rightarrow \forall h,\forall y, h(y) \notin Eval_{SQL}(Q[h(x)],h(D)) \\
		&\Rightarrow \forall h, \{y | h(y) \in Eval_{SQL}(Q[h(x)],h(D))\} = \emptyset \\
		&\Rightarrow \forall h, Eval_{SQL}(Q[h(x)],h(D) = \emptyset \mbox{ (by 3)} \\
		&\Rightarrow \forall h, h(x) \in Eval_{SQL}((\Sigma,R,notexists(Q),h(P)),h(D))\\
		&\Rightarrow  x \in cert_\bot((\Sigma,R,notexists(Q),P),D)
	\end{align*}
\end{proof}

\begin{proof}
	Assume (4).
	\\By induction ...
	\begin{align*}
		x \in posi_\bot((\Sigma,R,notexists(Q),P),D) &\Rightarrow \exists h, h(x) \in Eval_{SQL}((\Sigma,R,notexists(Q),P),h(D))  \\
		&\Rightarrow \exists h, Eval_{SQL}(Q[h(x)],h(D)) = \emptyset \\
		&\Rightarrow \{y | \forall g, g(y) \in Eval_{SQL}(Q[g(x)],g(D))\} = \emptyset \\
		&\Rightarrow Eval_{SQL}(Q^+[x],D) = \emptyset \mbox{ (by 4)}\\
		&\Rightarrow x \in Eval_{SQL}(\Sigma,R,notexists(Q^+),P),D) \\
		&\Rightarrow x \in Eval_{SQL}(\Sigma,R,notexists(Q),P)^?,D)
	\end{align*}
\end{proof}

