%!TEX root = main.tex

For now : 
I don't consider full-join.
To do : A lot :) 
Don't forget to demonstrate that u dont loose certain answer that "normal" evaluation would return.

\section{Preliminaries}

\begin{mydef}
	We denote the Set of well formed select query without agregation, full join and null test by $\llbracket SQL\rrbracket$
	\\We denote the Set of well formed select query without agregation and full join by $\llbracket SQL\rrbracket _\bot$
\end{mydef}

\begin{mydef}
Let's a Select query $Q \in \llbracket SQL\rrbracket$ a tuple $(\Sigma,R,H,P)$ such that
\begin{align*}
\Sigma & \subseteq \{r_i.a_i | \exists r_i \in R \land \exists a_i \in r_i \} \\
P & \subseteq \{p_i = r_j.a_j | r_j \notin R\} \mbox{ a set of external parameter.}\\
R & \mbox{ a set of relation.}\\
H &  \mbox{ belongs to the following grammar}\\
\end{align*}

\begin{align*}
H ::= &\ r_i.a_i = c_i \; |\; r_i.a_i \neq c_j \; |\; r_i.a_i = r_j.a_j \; |\;  r_i.a_i \neq r_j.a_j \;  |\; r_i.a_i = p_i\; |\; 
\\ &  exists(Q) \; |\; notexists(Q) \; |\; in(r_i.a_i,Q) \; |\; notin(r_i.a_i,Q) \; |\; 
\\ & H\land H \; |\; H \lor H 
\\
\end{align*}

\end{mydef}

\begin{mydef}
Let's a Select query $Q \in \llbracket SQL\rrbracket _\bot$ a tuple $(\Sigma,R,H,P)$ such that
\begin{align*}
\Sigma & \subseteq \{r_i.a_i | \exists r_i \in R \land \exists a_i \in r_i \} \\
P & \subseteq \{p_i = r_j.a_j | r_j \notin R\} \mbox{ a set of external parameter.}\\
R & \mbox{ a set of relation.}\\
H_\bot &  \mbox{ belongs to the following grammar}\\
\end{align*}

\begin{align*}
H_{\bot} ::= &\ r_i.a_i = c_i \; |\; r_i.a_i \neq c_j \; |\; r_i.a_i = r_j.a_j \; |\;  r_i.a_i \neq r_j.a_j \; |
\\&  r_i.a_i = p_i\; |\; null(r_i.a_i) \; |\;  const(r_i.a_i)\;
\\ &  exists(Q_{\bot}) \; |\; notexists(Q_{\bot}) \; |\; in(r_i.a_i,Q_{\bot}) \; |\; notin(r_i.a_i,Q_{\bot}) \; |\; 
\\ & H_{\bot}\land H_{\bot} \; |\; H_{\bot} \lor H_{\bot} 
\\
\end{align*}

%We denote by $\cF$ the set of formulas in \QFBILIA, by $\cT_{int}$ the set of integer terms, by $\cT_{ext}$ the set of extremum terms, and by $\cT_{bag}$ the set of multi-set terms.
\end{mydef}

We denote $(\Sigma,R,H,P)[x]$ the query $(\Sigma,R,H,P\cup x)$

\begin{myprop}
	$$\llbracket SQL\rrbracket \subset \llbracket SQL\rrbracket _\bot$$
\end{myprop}
\begin{proof}
	immediate i guess ?
\end{proof}

\begin{myex}

\begin{verbatim}
SELECT F1.titre, F2.titre FROM Film as F1, Film as F2 WHERE NOT EXISTS 
	(SELECT id_production FROM Production WHERE Production.id_film = F1.id_film 
	AND id_production NOT IN 		
		(SELECT id_production FROM Production WHERE Production.id_film = F2.id_film))
and NOT EXISTS 
	(SELECT id_production FROM Production WHERE Production.id_film = F2.id_film 
	AND id_production NOT IN 
		(SELECT id_production FROM Production WHERE Production.id_film = F1.id_film));
\end{verbatim}
--
\\$Q = (\Sigma,R,H)$
\\$\Sigma = \{F1.titre, F2.titre\}$
\\$R = \{F1,F2\}$
\\$H = notexists(Q_1) \land notexists(Q_2)$
\\$P = \emptyset$

--
\\$Q_1 = (\Sigma_1,R_1,H_1)$
\\$\Sigma_1 = \{id\_production\}$
\\$R_1 = \{Production\}$
\\$H_1 = Production.id\_film = F1.id\_film \land notin(id\_production,Q_{11})$
\\$P =\{ F1.id\_film,F2.id_film\}$

--
\\$Q_{11} = (\Sigma_{11},R_{11},H_{11})$
\\$\Sigma_{11} = \{id\_production\}$
\\$R_{11} = \{Production\}$
\\$H_{11} =  Production.id\_film = F2.id\_film$
\\$P =\{ F1.id\_film,F2.id_film\}$

--
\\$Q_2 = (\Sigma_2,R_2,H_2)$
\\$\Sigma_2 = \{id\_production\}$
\\$R_2 = \{Production\}$
\\$H_2 = Production.id\_film = F2.id\_film \land notin(id\_production,Q_{21})$
\\$P =\{ F1.id\_film,F2.id_film\}$

--
\\$Q_{21} = (\Sigma_{21},R_{21},H_{21})$
\\$\Sigma_{21} = \{id\_production\}$
\\$R_{21} = \{Production\}$
\\$H_{21} =  Production.id\_film = F1.id\_film$
\\$P =\{ F1.id\_film,F2.id_film\}$

\end{myex}


\subsection{Syntaxic Sugar}

NO BAGS FOR NOW. (Only a sketch to keep it in mind)
\\AND WRONG
\begin{myprop}
$$ Eval_{SQL}((\Sigma_0, R_0 \cup (\Sigma_1,R_1,H_1,P_1) ,H_0,P_0),D) = Eval_{SQL}((\Sigma_0, R_0 \cup R_1 ,H_0 \land H_1,P_0 \cup P_1),D)$$
$$ Eval_{SQL}((\Sigma_1,R_1,H_1,P_1),D) \cup Eval_{SQL}((\Sigma_2,R_2,H_2,P_2),D) = Eval_{SQL}((\Sigma_1,R_1\cup R_2,H_1\lor H_2,P_1\cup P_2),D)$$ 
$$ Eval_{SQL}((\Sigma_1,R_1,H_1,P_1),D) \cap Eval_{SQL}((\Sigma_2,R_2,H_2,P_2),D) = Eval_{SQL}((\Sigma_1,R_1\cup R_2,H_1\land H_2,P_1\cup P_2),D)$$ 
$$ Eval_{SQL}((\Sigma_1,R_1,H_1,P_1),D) \setminus Eval_{SQL}((\Sigma_2,R_2,H_2,P_2),D) = Eval_{SQL}((\Sigma_1,R_1,H_1\land notexists((\Sigma_2,R_2,H_2 \land (\Sigma_1 = \Sigma_2) ,P_2)),P_1),D)$$ 
$$Eval_{SQL}((\Sigma_0,R_0,notin(r_i.a_i,(\Sigma_1,R_1,H_1,P_1)),P_0),D) = Eval_{SQL}((\Sigma_0,R_0,notexists(\Sigma_1,R_1,H_1\land r_i.a_i = \Sigma_1,P_1),P_0),D)$$
$$Eval_{SQL}((\Sigma_0,R_0,in(r_i.a_i,(\Sigma_1,R_1,H_1,P_1)),P_0),D) = Eval_{SQL}((\Sigma_0,R_0,exists(\Sigma_1,R_1,H_1\land r_i.a_i = \Sigma_1,P_1),P_0),D)$$


\end{myprop}
\begin{proof}
	To do ..
\end{proof}


