\section{Removing useless null check}
The translation $Q \rightarrow Q^+$ has an heavy cost has explained in the paper ..., in order to remove some useless null test we offer an optimization.

\begin{mydef}
	For each Query and nested Query we maintain a set of attributes that have to be not null in order for the query to be true resp. false we denote this set $\bot^T_{Q}$ resp.$\bot^F_{Q}$.
\end{mydef} 

%Contraintes montantes
\begin{mydef}
	\begin{align*}
		\bot^T_{(\Sigma,R,H_1 \land H_2,P)} & = \bot^T_{(\Sigma,R,H_1,P)} \cup \bot^T_{(\Sigma,R,H_2,P)} \\
		\bot^T_{(\Sigma,R,H_1 \lor H_2,P)} & = \bot^T_{(\Sigma,R,H_1,P)} \cap \bot^T_{(\Sigma,R,H_2,P)} \\
		\bot^T_{(\Sigma,R,r_i.a_i = c_i,P)} & = \{r_i.a_i\} \\
		\bot^T_{(\Sigma,R,r_i.a_i \neq c_i,P)} & = \{r_i.a_i\} \\
		\bot^T_{(\Sigma,R,r_i.a_i = r_j.a_j,P)} & = \{r_i.a_i,r_j.a_j\} \\
		\bot^T_{(\Sigma,R,r_i.a_i \neq r_j.a_j,P)} & = \{r_i.a_i,r_j.a_j\} \\
		\bot^T_{(\Sigma,R,r_i.a_i = p_i,P)} & = \{r_i.a_i,p_i\} \\
		\bot^T_{(\Sigma,R,r_i.a_i \neq p_i,P)} & = \{r_i.a_i,p_i\} \\
		\bot^T_{(\Sigma,R,null(r_i.a_i),P)} & = \emptyset \\
		\bot^T_{(\Sigma,R,const(r_i.a_i),P)} & = \{r_i.a_i\} \\
		\bot^T_{(\Sigma,R,exists(Q),P)} & = \bot^T_{Q[?]} \\
		\bot^T_{(\Sigma,R,notexists(Q),P)} & = \bot^F_{Q[?]}\\
	\end{align*}
	
	\begin{align*}
		\bot^F_{(\Sigma,R,H_1 \land H_2,P)} & = \bot^F_{(\Sigma,R,H_1,P)} \cap \bot^F_{(\Sigma,R,H_2,P)} \\
		\bot^F_{(\Sigma,R,H_1 \lor H_2,P)} & = \bot^F_{(\Sigma,R,H_1,P)} \cup \bot^F_{(\Sigma,R,H_2,P)} \\
		\bot^F_{(\Sigma,R,r_i.a_i = c_i,P)} & =\emptyset \\
		\bot^F_{(\Sigma,R,r_i.a_i \neq c_i,P)} & = \emptyset \\
		\bot^F_{(\Sigma,R,r_i.a_i = r_j.a_j,P)} & = \emptyset \\
		\bot^F_{(\Sigma,R,r_i.a_i \neq r_j.a_j,P)} & = \emptyset \\
		\bot^F_{(\Sigma,R,r_i.a_i = p_i,P)} & = \emptyset\\
		\bot^F_{(\Sigma,R,r_i.a_i \neq p_i,P)} & = \emptyset \\
		\bot^F_{(\Sigma,R,null(r_i.a_i),P)} & = \emptyset \\
		\bot^F_{(\Sigma,R,const(r_i.a_i),P)} & = \emptyset \\
		\bot^F_{(\Sigma,R,exists(Q),P)} & = \bot^F_{Q[?]} \\
		\bot^F_{(\Sigma,R,notexists(Q),P)} & = \bot^T_{Q[?]}\\
	\end{align*}
\end{mydef}

\begin{myprop}
	$$x \in Eval_{SQL}(Q_*,D)  \Rightarrow \forall r_i.a_i \in \bot^T_Q, x[r_i.a_i] \neq \bot$$
	$$x \notin Eval_{SQL}(Q_*,D)  \Rightarrow \forall r_i.a_i \in \bot^F_Q, x[r_i.a_i] \neq \bot$$
\end{myprop}

\begin{proof}
			
\end{proof}


\begin{mydef}
	
	\begin{align*}
		nested^+(H_1\land H_2) & = \{H_1 \land H_2\}  \cup nested^+(H_1) \cup nested^+(H_2) \\
		nested^+(H_1\lor H_2) & = \{H_1 \lor H_2\}  \cup nested^+(H_1) \cup nested^+(H_2) \\
		nested^+(r_i.a_i = c_i) & = \{r_i.a_i = c_i\} \\
		nested^+(r_i.a_i \neq c_i) & = \{r_i.a_i \neq c_i\} \\
		nested^+(r_i.a_i = r_j.a_j) & = \{r_i.a_i = r_j.a_j\} \\
		nested^+(null(r_i.a_i)) & = \{null(r_i.a_i)\} \\
		nested^+(const(r_i.a_i)) & = \{const(r_i.a_i)\} \\
		nested^+(exists(Q)) & = \{exists(Q)\} \cup nested^+(Q) \\
		nested^+(notexists(Q)) & = \{notexists(Q)\} \cup nested^-(Q) \\
	\end{align*}
	
	\begin{align*}
		nested^-(H_1\land H_2) & =nested^-(H_1) \cup nested^-(H_2) \\
		nested^-(H_1\lor H_2) & =  nested^-(H_1) \cup nested^-(H_2) \\
		nested^-(r_i.a_i = c_i) & = \emptyset \\
		nested^-(r_i.a_i \neq c_i) & = \emptyset \\
		nested^-(r_i.a_i = r_j.a_j) & = \emptyset \\
		nested^-(null(r_i.a_i)) & = \emptyset \\
		nested^-(const(r_i.a_i)) & = \emptyset \\
		nested^-(exists(Q)) & =nested^-(Q) \\
		nested^-(notexists(Q)) & = nested^+(Q) \\
	\end{align*}
	
	\begin{align*}
		nested(Q) & = nested^-(Q) \cup nested^+(Q)
	\end{align*}
\end{mydef}

\begin{mydef}
	\begin{align*}
		notexists(Q')^\bot_Q & \rightarrow notexists(Q'^\bot_Q)
		\\exists(Q')^\bot_Q & \rightarrow exists(Q'^\bot_Q)
	\end{align*}
\end{mydef}

\begin{mydef}
	\begin{align*}
		(\Sigma,R,H \lor null(r_i.a_i),P)^\bot_Q & \rightarrow (\Sigma,R,H^\bot_{Q},P) \\
		& \mbox{if } \exists Q' \in nested^+(Q), (H\lor null(r_i.a_i)) \in nested(Q'), r_i.a_i \in \bot^T_{Q'} \\
		& \mbox{if } \exists Q' \in nested^-(Q), (H\lor null(r_i.a_i)) \in nested(Q'), r_i.a_i \in \bot^F_{Q'}
	\end{align*}
\end{mydef}



\begin{myprop}
	$$Eval_{SQL}(Q,D) = Eval_{SQL}(Q^\bot_Q,D)$$
\end{myprop}

\begin{proof}
	
	\begin{mydef}
		\begin{align*}
			(\Sigma,R,H \lor null(r_i.a_i),P)^{\bot^F}_Q & \rightarrow (\Sigma,R,H^{\bot^F}_{Q},P) \\
			& \mbox{if } \exists Q' \in nested^-(Q), (H\lor null(r_i.a_i)) \in nested(Q'), r_i.a_i \in \bot^T_{Q'} \\
			& \mbox{if } \exists Q' \in nested^+(Q), (H\lor null(r_i.a_i)) \in nested(Q'), r_i.a_i \in \bot^F_{Q'}
		\end{align*}
	\end{mydef}
	
	\begin{myprop}
		$$\forall Q' \in nested^+(Q), Eval(Q,D) = Eval(Q^\bot_{Q'},D)$$
	\end{myprop}
	\begin{myprop}
		$$\forall Q' \in nested^-(Q), Eval(Q,D) = Eval(Q^{\bot^F}_{Q'},D)$$
	\end{myprop}
	
	\begin{proof}
		Assume (10).
		\\By Induction ...
		\\$H_1 \land H_2 \in nested^+(Q)$
		\\$\exists r_i.a_i \in (\bot^T_{H_1} \setminus \bot^T_{H_2}) \land (H\lor null(r_i.a_i)\in nested(H_2)$
		\\Then if $x[r_i.a_i] = \bot$, $Eval(H^T_{2,H_2},D,x)$ might be different from $Eval(H^T_{2,H_1\land H_2},D,x)$
	\end{proof}
	
	
\end{proof}

\begin{myprop}
	
\end{myprop}
